QueueingSystems.v
@@ -1,10 +1,6 @@
 Require Import Coq.Lists.List.
 Import ListNotations.
 
-Set Implicit Arguments.
-Unset Strict Implicit.
-Unset Printing Implicit Defensive.
-
 Require Import DFA.
 
 Require Export Arith_base.
@@ -12,12 +8,12 @@ Require Import BinPos BinInt BinNat Pnat Nnat.
 Require Import Omega.
 Local Open Scope Z_scope.
 
-Inductive events {E : Type} : Type :=
+Inductive event {E : Type} : Type :=
   | add
   | rem
   | other (e : E).
 
-Fixpoint buffer_count {E : Type} (w : list (@events E)) : Z :=
+Fixpoint buffer_count {E : Type} (w : list (@event E)) : Z :=
   match w with
   | [] => 0
   | add::w' => buffer_count w' + 1
@@ -25,10 +21,10 @@ Fixpoint buffer_count {E : Type} (w : list (@events E)) : Z :=
   | _::w' => buffer_count w'
   end.
 
-Definition upper_bound {Q E : Type} (g : dfa Q (@events E)) (n : Z) :=
+Definition upper_bound {Q E : Type} (g : dfa Q (@event E)) n :=
   forall w, w ==> g -> buffer_count w <= n.
 
-Lemma buffer_add: forall (E : Type) (w : list (@events E)),
+Lemma buffer_add: forall (E : Type) (w : list (@event E)),
   buffer_count (w ++ [add]) = buffer_count w + 1.
 Proof.
   intros E w.
@@ -40,7 +36,7 @@ Proof.
     + omega.
 Qed.
 
-Lemma buffer_rem: forall (E : Type) (w : list (@events E)),
+Lemma buffer_rem: forall (E : Type) (w : list (@event E)),
   buffer_count (w ++ [rem]) = buffer_count w - 1.
 Proof.
   intros E w.
@@ -52,7 +48,7 @@ Proof.
     + omega.
 Qed.
 
-Lemma buffer_other: forall (E : Type) (w : list (@events E)) (e : E),
+Lemma buffer_other: forall (E : Type) (w : list (@event E)) (e : E),
   buffer_count (w ++ [other e]) = buffer_count w.
 Proof.
   intros E w c.
@@ -61,8 +57,8 @@ Proof.
   - simpl. rewrite IH. reflexivity.
 Qed.
 
-Lemma extended_delta__delta: forall (Q E : Type) (g : dfa Q E) (q : Q) (e : E),
-  extended_delta g (state q) [e] = g.(delta) q e.
+Lemma extended_delta__delta: forall (Q E : Type) (g : dfa Q E) q e,
+  extended_delta g (proper_state q) [e] = (delta g) q e.
 Proof.
   intros Q E g q e.
   simpl.
@@ -72,13 +68,13 @@ Proof.
 Qed.
 
 Lemma buffer_count_leq_f:
-  forall (Q E : Type) (g : dfa Q (@events E)) (f : @states Q->Z),
-    (f(state g.(initial_state)) = 0 /\
+  forall (Q E : Type) (g : dfa Q (@event E)) (f : @state Q->Z),
+    (f(proper_state (initial_state g)) = 0 /\
       forall (q : Q),
-        f(g.(delta) q add) >= f(state q) + 1 /\
-        f(g.(delta) q rem) >= f(state q) - 1 /\
-        (forall (e : E), f(g.(delta) q (other e)) >= f(state q))
-    ) -> (forall w, w ==> g -> buffer_count w <= f (extended_delta g (state g.(initial_state)) w)).
+        f((delta g) q add) >= f(proper_state q) + 1 /\
+        f((delta g) q rem) >= f(proper_state q) - 1 /\
+        (forall (e : E), f((delta g) q (other e)) >= f(proper_state q))
+    ) -> (forall w, w ==> g -> buffer_count w <= f (extended_delta g (proper_state (initial_state g)) w)).
 Proof.
   intros Q E g f H0 w H2.
   destruct H0 as [H0 H1].
@@ -89,61 +85,61 @@ Proof.
     apply IHw in H3.
     destruct e.
     + rewrite buffer_add.
-      assert (f (extended_delta g (state (initial_state g)) (w)) + 1 <= f (extended_delta g (state (initial_state g)) (w ++ [add]))).
-      { rewrite dist_extended_delta. remember (extended_delta g (state (initial_state g)) w) as q eqn:eq_q. destruct q.
+      assert (f (extended_delta g (proper_state (initial_state g)) (w)) + 1 <= f (extended_delta g (proper_state (initial_state g)) (w ++ [add]))).
+      { rewrite dist_extended_delta. remember (extended_delta g (proper_state (initial_state g)) w) as q eqn:eq_q. destruct q.
         - apply prefix_closed in H2. unfold in_language in H2. unfold not in H2. symmetry in eq_q. apply H2 in eq_q.
           destruct eq_q.
-        - rewrite extended_delta__delta. assert (f (delta g q add) >= f (state q) + 1).
+        - rewrite extended_delta__delta. assert (f (delta g q add) >= f (proper_state q) + 1).
           { apply H1. }
           omega. }
       omega.
     + rewrite buffer_rem.
-      assert (f (extended_delta g (state (initial_state g)) (w)) - 1 <= f (extended_delta g (state (initial_state g)) (w ++ [rem]))).
-      { rewrite dist_extended_delta. remember (extended_delta g (state (initial_state g)) w) as q eqn:eq_q. destruct q.
+      assert (f (extended_delta g (proper_state (initial_state g)) (w)) - 1 <= f (extended_delta g (proper_state (initial_state g)) (w ++ [rem]))).
+      { rewrite dist_extended_delta. remember (extended_delta g (proper_state (initial_state g)) w) as q eqn:eq_q. destruct q.
         - apply prefix_closed in H2. unfold in_language in H2. unfold not in H2. symmetry in eq_q. apply H2 in eq_q.
           destruct eq_q.
-        - rewrite extended_delta__delta. assert (f (delta g q rem) >= f (state q) - 1).
+        - rewrite extended_delta__delta. assert (f (delta g q rem) >= f (proper_state q) - 1).
           { apply H1. }
           omega. }
       omega.
     + rewrite buffer_other.
-      assert (f (extended_delta g (state (initial_state g)) (w)) <= f (extended_delta g (state (initial_state g)) (w ++ [other e]))).
-      { rewrite dist_extended_delta. remember (extended_delta g (state (initial_state g)) w) as q eqn:eq_q. destruct q.
+      assert (f (extended_delta g (proper_state (initial_state g)) (w)) <= f (extended_delta g (proper_state (initial_state g)) (w ++ [other e]))).
+      { rewrite dist_extended_delta. remember (extended_delta g (proper_state (initial_state g)) w) as q eqn:eq_q. destruct q.
         - apply prefix_closed in H2. unfold in_language in H2. unfold not in H2. symmetry in eq_q. apply H2 in eq_q.
           destruct eq_q.
-        - rewrite extended_delta__delta. assert (f (delta g q (other e)) >= f (state q)).
+        - rewrite extended_delta__delta. assert (f (delta g q (other e)) >= f (proper_state q)).
           { apply H1. }
           omega. }
       omega.
 Qed.
 
 Theorem th1:
-  forall (Q E : Type) (g : dfa Q (@events E)) (n : Z),
-    (exists (f : @states Q->Z), f(state g.(initial_state)) = 0 /\
+  forall (Q E : Type) (g : dfa Q (@event E)) n,
+    (exists (f : @state Q->Z), f(proper_state (initial_state g)) = 0 /\
       forall (q : Q),
-        f(state q) <= n /\
-        f(g.(delta) q add) >= f(state q) + 1 /\
-        f(g.(delta) q rem) >= f(state q) - 1 /\
-        (forall (e : E), f(g.(delta) q (other e)) >= f(state q))
+        f(proper_state q) <= n /\
+        f((delta g) q add) >= f(proper_state q) + 1 /\
+        f((delta g) q rem) >= f(proper_state q) - 1 /\
+        (forall (e : E), f((delta g) q (other e)) >= f(proper_state q))
     ) -> upper_bound g n.
 Proof.
   unfold upper_bound.
   intros Q E g n H0 w H2.
   destruct H0 as [f [H0 H1]].
   induction w as [|e w IHw] using @rev_ind.
-  - assert (H3 : f (state (initial_state g)) <= n).
+  - assert (H3 : f (proper_state (initial_state g)) <= n).
     { apply H1. }
     rewrite H0 in H3.
     apply H3.
   - destruct e.
-    + assert (H3 : forall w, w ==> g -> buffer_count w <= f (extended_delta g (state g.(initial_state)) w)).
+    + assert (H3 : forall w, w ==> g -> buffer_count w <= f (extended_delta g (proper_state (initial_state g)) w)).
       { apply buffer_count_leq_f. split.
           - apply H0. 
           - intros H3. apply H1. }
-      assert (buffer_count (w ++ [add]) <= f (extended_delta g (state (initial_state g)) (w ++ [add]))).
+      assert (buffer_count (w ++ [add]) <= f (extended_delta g (proper_state (initial_state g)) (w ++ [add]))).
       { apply H3. apply H2. }
-      assert (f (extended_delta g (state (initial_state g)) (w ++ [add])) <= n).
-      { remember (extended_delta g (state (initial_state g)) (w ++ [add])) as q eqn:eq_q.
+      assert (f (extended_delta g (proper_state (initial_state g)) (w ++ [add])) <= n).
+      { remember (extended_delta g (proper_state (initial_state g)) (w ++ [add])) as q eqn:eq_q.
         destruct q.
         - unfold in_language in H2. unfold not in H2. symmetry in eq_q. apply H2 in eq_q. destruct eq_q.
         - apply H1. }
@@ -156,27 +152,27 @@ Proof.
 Qed.
 
 Theorem th2:
-  forall (Q E : Type) (g : dfa Q (@events E)) (n : Z),
+  forall (Q E : Type) (g : dfa Q (@event E)) n,
     upper_bound g n ->
-    (exists (f : @states Q->Z), f(state g.(initial_state)) = 0 /\
+    (exists (f : @state Q->Z), f(proper_state (initial_state g)) = 0 /\
       forall (q : Q),
-        f(state q) <= n /\
-        f(g.(delta) q add) >= f(state q) + 1 /\
-        f(g.(delta) q rem) >= f(state q) - 1 /\
-        (forall (e : E), f(g.(delta) q (other e)) >= f(state q))
+        f(proper_state q) <= n /\
+        f((delta g) q add) >= f(proper_state q) + 1 /\
+        f((delta g) q rem) >= f(proper_state q) - 1 /\
+        (forall (e : E), f((delta g) q (other e)) >= f(proper_state q))
     ).
 Proof.
 (* FICA PARA O TCC 2 ;-) *)
 Admitted.
 
 Theorem th12:
-  forall (Q E : Type) (g : dfa Q (@events E)) (n : Z),
-    (exists (f : @states Q->Z), f(state g.(initial_state)) = 0 /\
+  forall (Q E : Type) (g : dfa Q (@event E)) n,
+    (exists (f : @state Q->Z), f(proper_state (initial_state g)) = 0 /\
       forall (q : Q),
-        f(state q) <= n /\
-        f(g.(delta) q add) >= f(state q) + 1 /\
-        f(g.(delta) q rem) >= f(state q) - 1 /\
-        (forall (e : E), f(g.(delta) q (other e)) >= f(state q))
+        f(proper_state q) <= n /\
+        f((delta g) q add) >= f(proper_state q) + 1 /\
+        f((delta g) q rem) >= f(proper_state q) - 1 /\
+        (forall (e : E), f((delta g) q (other e)) >= f(proper_state q))
     ) <-> upper_bound g n.
 Proof.
   split.
@@ -185,13 +181,13 @@ Proof.
 Qed.
 
 Theorem upper_bound_geq_0:
-  forall (Q E : Type) (g : dfa Q (@events E)) n,
+  forall (Q E : Type) (g : dfa Q (@event E)) n,
     upper_bound g n -> n >= 0.
 Proof.
   intros Q E g n H.
   apply th12 in H.
   destruct H as [f H], H as [H H0].
-  assert (f (state (initial_state g)) <= n).
+  assert (f (proper_state (initial_state g)) <= n).
   { apply H0. }
   omega.
 Qed.
